\documentclass[letterpaper]{article}
\usepackage[letterpaper,margin=1in,footskip=0.25in]{geometry}
\usepackage[utf8]{inputenc}
\usepackage{amsmath}
\usepackage{amsthm}
\usepackage{amssymb, pifont}
\usepackage{mathrsfs}
\usepackage{enumitem}
\usepackage{fancyhdr}
\usepackage{hyperref}

\pagestyle{fancy}
\fancyhf{}
\rhead{MAT 257}
\lhead{Assignment 15}
\rfoot{Page \thepage}

\setlength\parindent{24pt}
\renewcommand\qedsymbol{$\blacksquare$}

\DeclareMathOperator{\T}{\mathcal{T}}
\DeclareMathOperator{\V}{\mathcal{V}}
\DeclareMathOperator{\U}{\mathcal{U}}
\DeclareMathOperator{\Prt}{\mathbb{P}}
\DeclareMathOperator{\R}{\mathbb{R}}
\DeclareMathOperator{\N}{\mathbb{N}}
\DeclareMathOperator{\Z}{\mathbb{Z}}
\DeclareMathOperator{\Q}{\mathbb{Q}}
\DeclareMathOperator{\C}{\mathbb{C}}
\DeclareMathOperator{\ep}{\varepsilon}
\DeclareMathOperator{\identity}{\mathbf{0}}
\DeclareMathOperator{\card}{card}
\newcommand{\suchthat}{;\ifnum\currentgrouptype=16 \middle\fi|;}

\newtheorem{lemma}{Lemma}

\newcommand{\bd}{\partial}
\newcommand{\tr}{\mathrm{tr}}
\newcommand{\ra}{\rightarrow}
\newcommand{\lan}{\langle}
\newcommand{\ran}{\rangle}
\newcommand{\norm}[1]{\left\lVert#1\right\rVert}
\newcommand{\inn}[1]{\lan#1\ran}
\newcommand{\ol}{\overline}
\begin{document}
\noindent Q4: We first verify that $d^2\omega=0$. We compute that 
\begin{align*}
d(d\omega) & = d(\sum_{i=1}^3 dx_i \wedge \frac{\bd \omega}{\bd x_i})
\\ & = d(dx \wedge(ydx) + dy \wedge(x dx -z dz) + dz \wedge(-y dz) )
\\ & = d(-x dx \wedge dy - z dy \wedge dz )
\\ & = d(-x dx\wedge dy) - d(zdy\wedge dz)
\\ & = dx \wedge ( -dx \wedge dy) - dz \wedge (dy \wedge dz)
\\ & =0
\end{align*} Unsurprisingly $d^2\omega=0$. We now will verify that $d(\omega \wedge \eta) = d\omega \wedge \eta - \omega \wedge d\eta$. We first compute the left side. 
\begin{align*}
d(\omega \wedge \eta) &= d((-xy^2z^2-3x)dx\wedge dy + (2x^2+xz)dx\wedge dz + (6x-y^2z^3)dy\wedge dz)
\\ & = 6 dx \wedge dy \wedge dz -(2x^2+xz)dx \wedge dy \wedge dz - 2xy^2z dx \wedge dy \wedge dz
\\ & = (6-2x^2-xz-2xy^2z)dx\wedge dy\wedge dz
\end{align*}
We will now compute the right side: 
\begin{align*}
d\omega \wedge \eta - \omega \wedge d\eta & = (-x dx\wedge dy -z dy \wedge dz)\wedge(xdx - yz^2dy + 2x dz) - (xy dx + 3dy - yzdz)\wedge(2dx \wedge dz + 2yz dy \wedge dz)
\\ & = (-2x^2-xz)dx \wedge dy \wedge dz - (2xy^2z-6)dx\wedge dy \wedge dz
\\ & = (6-2x^2-xz-2xy^2z)dx\wedge dy\wedge dz
\end{align*}Once again we are not surprised to see that indeed $d(\omega \wedge \eta) = d\omega \wedge \eta - \omega \wedge d\eta$. 
\end{document}