\documentclass[12pt, a4paper]{article}
\usepackage[lmargin =0.5 in, 
rmargin=0.5in, 
tmargin=1in,
bmargin=0.5in]{geometry}
\geometry{letterpaper}
\usepackage{tikz-cd}
\usepackage{amsmath}
\usepackage{amssymb}
\usepackage{blindtext}
\usepackage{titlesec}
\usepackage{enumitem}
\usepackage{fancyhdr}
\usepackage{amsthm}
\usepackage{graphicx}
\usepackage{cool}
\usepackage{thmtools}
\usepackage{hyperref}
\graphicspath{ }					%path to an image

%-------- sexy font ------------%
%\usepackage{libertine}
%\usepackage{libertinust1math}

%\usepackage{mlmodern}				% very nice and classic
%\usepackage[utopia]{mathdesign}
%\usepackage[T1]{fontenc}


\usepackage{mlmodern}
\usepackage{eulervm}
%\usepackage{tgtermes} 				%times new roman
%-------- sexy font ------------%


% Problem Styles
%====================================================================%


\newtheorem{problem}{Problem}


\theoremstyle{definition}
\newtheorem{thm}{Theorem}
\newtheorem{lemma}{Lemma}
\newtheorem{prop}{Proposition}
\newtheorem{cor}{Corollary}
\newtheorem{fact}{Fact}
\newtheorem{defn}{Definition}
\newtheorem{example}{Example}
\newtheorem{question}{Question}

\newtheorem{manualprobleminner}{Problem}

\newenvironment{manualproblem}[1]{%
	\renewcommand\themanualprobleminner{#1}%
	\manualprobleminner
}{\endmanualprobleminner}

\newcommand{\penum}{ \begin{enumerate}[label=\bf(\alph*), leftmargin=0pt]}
	\newcommand{\epenum}{ \end{enumerate} }

% Math fonts shortcuts
%====================================================================%

\newcommand{\ring}{\mathcal{R}}
\newcommand{\N}{\mathbb{N}}                           % Natural numbers
\newcommand{\Z}{\mathbb{Z}}                           % Integers
\newcommand{\R}{\mathbb{R}}                           % Real numbers
\newcommand{\C}{\mathbb{C}}                           % Complex numbers
\newcommand{\F}{\mathbb{F}}                           % Arbitrary field
\newcommand{\Q}{\mathbb{Q}}                           % Arbitrary field
\newcommand{\PP}{\mathcal{P}}                         % Partition
\newcommand{\M}{\mathcal{M}}                         % Mathcal M
\newcommand{\eL}{\mathcal{L}}                         % Mathcal L
\newcommand{\T}{\mathbb{T}}                         % Mathcal T
\newcommand{\U}{\mathcal{U}}                         % Mathcal U\\
\newcommand{\V}{\mathcal{V}}                         % Mathcal V

% symbol shortcuts
%====================================================================%

\newcommand{\bd}{\partial}
\newcommand{\grad}{\nabla}
\newcommand{\lam}{\lambda}
\newcommand{\imp}{\implies}
\newcommand{\all}{\forall}
\newcommand{\exs}{\exists}
\newcommand{\delt}{\delta}
\newcommand{\ep}{\varepsilon}
\newcommand{\ra}{\rightarrow}
\newcommand{\vph}{\varphi}

\newcommand{\ol}{\overline}
\newcommand{\f}{\frac}
\newcommand{\lf}{\lfrac}
\newcommand{\df}{\dfrac}

% bracketting shortcuts
%====================================================================%
\newcommand{\abs}[1]{\left| #1 \right|}
\newcommand{\babs}[1]{\Big|#1\Big|}
\newcommand{\bound}{\Big|}
\newcommand{\BB}[1]{\left(#1\right)}
\newcommand{\dd}{\mathrm{d}}
\newcommand{\artanh}{\mathrm{artanh}}
\newcommand{\Med}{\mathrm{Med}}
\newcommand{\Cov}{\mathrm{Cov}}
\newcommand{\Corr}{\mathrm{Corr}}
\newcommand{\tr}{\mathrm{tr}}
\newcommand{\Range}[1]{\mathrm{range}(#1)}
\newcommand{\Null}[1]{\mathrm{null}(#1)}
\newcommand{\lan}{\langle}
\newcommand{\ran}{\rangle}
\newcommand{\norm}[1]{\left\lVert#1\right\rVert}
\newcommand{\inn}[1]{\lan#1\ran}
\newcommand{\op}[1]{\operatorname{#1}}
\newcommand{\bmat}[1]{\begin{bmatrix}#1\end{bmatrix}}
\newcommand{\pmat}[1]{\begin{pmatrix}#1\end{pmatrix}}
\newcommand{\vmat}[1]{\begin{vmatrix}#1\end{vmatrix}}

\newcommand{\amogus}{{\bigcap}\kern-0.8em\raisebox{0.3ex}{$\subset$}}
\newcommand{\Note}{\textbf{Note: }}
\newcommand{\Aside}{{\bf Aside: }}
%restriction
%\newcommand{\op}[1]{\operatorname{#1}}
%\newcommand{\done}{$$\mathcal{QED}$$}

%====================================================================%


\setlength{\parindent}{0pt}      	% No paragraph indentations
\pagestyle{fancy}
\fancyhf{}							% fancy header

\setcounter{secnumdepth}{0}			% sections are numbered but numbers do not appear
\setcounter{tocdepth}{2} 			% no subsubsections in toc

%template
%====================================================================%
%\begin{manualproblem}{1}
%Spivak.
%\end{manualproblem}

%\begin{proof}[Solution]
%\end{proof}

%----------- or -----------%

%\begin{problem} 		
%\end{problem}	

%\penum
%	\item
%\epenum
%====================================================================%


\newcommand{\Course}{APM462}
\newcommand{\hwNumber}{1}

%preamble

\title{}
\author{A.N.}
\date{\today}
\lhead{\Course A\hwNumber}
\rhead{\thepage}
%\cfoot{\thepage}


%====================================================================%
\begin{document}



\begin{problem}
\end{problem}
Suppose that $f$ continuous at $a$ and $g$ continuous at $f(a)$. Recall that for every $\ep_f$ there is a $\delta_f$ so that 
$\norm{x-a}< \delta_f$ implies that $\norm{f(a) - f(x)}<\epsilon_f$. Similarly for any $\ep_g>0$ we have a $\delta_g>0$ so that $\norm{f(a) - y} <\delta_g$ implies that $\norm{g(f(a)) - g(y)} < \ep_g$. We wish to show the same is true for $g\circ f$. Given $\ep >0$, we choose $\delta$ in the following way. Select $\delta_g $ for $y = f(x)$ from continuity of $g$. Then take $\ep_f = \delta_g$ and choose $\delta = \delta_f$ satisfying continuity of $f$ at $a$. This indeed works since: 
$$\norm{a - x} < \delta = \delta_f \implies \norm{f(a) - f(x)}< \ep_f = \delta_g \implies  \norm{g(f(a)) - g(f(x))} < \ep.$$\
Thus the composition of two continuous functions is continuous.   
\newpage
\begin{problem}
\end{problem}
Consider the following function:
$$f(x) = 
\begin{cases}
	 \frac{(x-1)(x+1)}{x^2} & x\in \Q \\
	0 & x\in \R \setminus \Q , x=0
\end{cases}$$
We claim that it is continuous at only $-1,1$. First at $x=1$ we have that $f(1) = 0$. We wish to find a $\delta$ so that $|f(x)|<\ep$ whenever $|1-x|<\delta$. Instead consider the function $g(x) = \frac{(x-1)(x+1)}{x^2}$. This is continuous on $\R \setminus\{0\}$ and agrees with $f$ on $\Q$. At $x=1$ for $\ep_g>0$ take $\delta_g$ so that the condition for continuity for $g$ at $x=1$ is satisfied. For $f$ taking $\delta = \delta_g$ for the same choice of $\ep$ will work, since $|f(x)| \leq |g(x)|$. Similarly this holds at $x=-1$. Away from $x=1, x=-1$ we have that $f$ is discontinuous since $|f(x)| >0$ on $\Q$, a dense set, and $f(x) = 0$ on $\R \setminus \{0\}$. 
\newpage
\begin{problem}
\end{problem}
Let $g: \R \to \R^n$ and $f: \R^n \to \R$ be $C^1$. For simplicity, take $n=2$. We write $g(t) = (x(t), y(t))$.  We wish to compute the derivative of $\phi = f \circ g$. 
First note that $$\phi(t+h) - \phi(t) = \left[f(x(t+h) , y(t+h)) - f(x(t+h) , y(t)) \right] + \left[f(x(t+h) , y(t)) - f(x(t) , y(t))	\right].$$
We define $g_1(k) = f(x(t+h) , y(t+k))$ and $g_2 (h) = f(x(t+h) , y(t))$. By the mean value theorem on $\R$, there exists a $\theta_1, \theta_2$ so that:
$$f(x(t+h) , y(t+h)) - f(x(t+h) , y(t)) = h \frac{\partial f}{\partial y} \cdot \frac{\partial y}{\partial t}(t+\theta_1 h),$$
and 
$$f(x(t+h) , y(t)) - f(x(t) , y(t)) = h \frac{\partial f}{\partial x}\cdot \frac{\partial x}{\partial t}(t + \theta_2 h).$$
We now compute the derivative of $\phi$ as:
\begin{align*}
	\phi^\prime(t)= \lim_{h \to 0}\frac{\phi(t+h) - \phi(t)}{h} & = \lim_{h \to 0} \frac{h \frac{\partial f}{\partial y} \cdot \frac{\partial y}{\partial t}(t+\theta_1 h)+h \frac{\partial f}{\partial x}\cdot \frac{\partial x}{\partial t}(t + \theta_2 h)}{h} \tag{using above}
	\\ & = \lim_{h \to 0} \frac{\partial f}{\partial y} \cdot \frac{\partial y}{\partial t}(t+\theta_1 h) + \frac{\partial f}{\partial x}\cdot \frac{\partial x}{\partial t}(t + \theta_2 h)
	\\ & = \frac{\partial f}{\partial y} \cdot \frac{\partial y}{\partial t}(t) + \frac{\partial f}{\partial x}\cdot \frac{\partial x}{\partial t}(t ) \tag{by Continuity of the partials}
\end{align*}
\newpage
\begin{problem}
\end{problem}
\penum
\item We show that $\grad f(x) = A^T b$ satisfies the limit definition of the gradient. 
\begin{align*}
	\lim_{h \to 0} \frac{f(x+h) - f(x)- A^Tb \cdot h}{h} & = \lim_{h \to 0} \frac{b \cdot A(x+h) - b \cdot Ax - A^Tb \cdot h}{h}
	\\ & = \lim_{h \to 0} \frac{b \cdot Ax + b \cdot Ah - b \cdot Ax - b \cdot Ah}{h} \tag{since $A^Tb = b \cdot A$}
	\\ & = 0
\end{align*}
By uniqueness of the gradient we have that $\grad f(x) = b \cdot A^T$. 
\item We show that $\grad f (x) = (A+A^T)x$ satisfies the limit definition of the gradient. 
\begin{align*}
	\lim_{h \to 0} \frac{(x+h) \cdot A (x+h) - x \cdot A x - (A+ A^T)x\cdot h}{h}
	  &= \lim_{h \to 0}\frac{x \cdot A x + h \cdot Ax + x \cdot Ah + h \cdot A h - x \cdot Ax -(A+ A^T)x\cdot h }{h}
	  \\ & = \lim_{h \to 0} \frac{h \cdot A x + x \cdot Ah - (A+A^T)x \cdot h}{h}
\end{align*}
\epenum 
\newpage
\begin{problem}
\end{problem}
\newpage
\begin{problem}
\end{problem}
\newpage
\begin{problem}
\end{problem}
\newpage


\end{document}
