\documentclass[letterpaper]{article}
\usepackage[letterpaper,margin=1in,footskip=0.25in]{geometry}
\usepackage[utf8]{inputenc}
\usepackage{amsmath}
\usepackage{amsthm}
\usepackage{amssymb, pifont}
\usepackage{mathrsfs}
\usepackage{enumitem}
\usepackage{fancyhdr}
\usepackage{hyperref}

\pagestyle{fancy}
\fancyhf{}
\rhead{MAT 457}
\lhead{Assignment 3}
\rfoot{Page \thepage}

\setlength\parindent{24pt}
\renewcommand\qedsymbol{$\blacksquare$}

\DeclareMathOperator{\E}{\mathcal{E}}
\DeclareMathOperator{\M}{\mathcal{M}}
\DeclareMathOperator{\F}{\mathbb{F}}
\DeclareMathOperator{\T}{\mathcal{T}}
\DeclareMathOperator{\V}{\mathcal{V}}
\DeclareMathOperator{\U}{\mathcal{U}}
\DeclareMathOperator{\Prt}{\mathbb{P}}
\DeclareMathOperator{\R}{\mathbb{R}}
\DeclareMathOperator{\N}{\mathbb{N}}
\DeclareMathOperator{\Z}{\mathbb{Z}}
\DeclareMathOperator{\Q}{\mathbb{Q}}
\DeclareMathOperator{\C}{\mathbb{C}}
\DeclareMathOperator{\ep}{\varepsilon}
\DeclareMathOperator{\identity}{\mathbf{0}}
\DeclareMathOperator{\card}{card}
\newcommand{\suchthat}{;\ifnum\currentgrouptype=16 \middle\fi|;}

\newtheorem{lemma}{Lemma}

\newcommand{\tr}{\mathrm{tr}}
\newcommand{\ra}{\rightarrow}
\newcommand{\lan}{\langle}
\newcommand{\ran}{\rangle}
\newcommand{\norm}[1]{\left\lVert#1\right\rVert}
\newcommand{\inn}[1]{\lan#1\ran}
\newcommand{\ol}{\overline}
\newcommand{\ci}{i}
\begin{document}
\noindent
Q4: For $a,b\geq 0$, we consider $$a- |a-b|$$
We wish to bound it above and below. First note that by the triangle inequality we have that $$|a-b| \leq |a| + |b|$$ When we multiply by $-1$ and add $a$ to get that $$-b=a - |a| - |b| \leq a-|a-b|$$ 
We now wish to find an upper bound for $$a - |a-b|$$. If $a-b>0$, then $$a-|a-b| = a-(a-b) =b$$
If we have that $a-b<0$, then $$a-(-a+b) = 2a-b$$ Since $2a<2b$ we know that $2a-b <b$ and hence we conclude that $$ - b \leq a - |a-b|\leq b$$
Replacing $a = f_n$, $b = f$, we get that $$\int f_n - |f_n -f| \leq \int f$$
Applying the dominating convergence theorem, we have that $$\lim_{n\to \infty} \int f_n - |f_n - f| = \int \lim_{n \to \infty} f_n - \int \lim_{n \to \infty} |f_n - f| = \int f$$

\end{document}