\documentclass[letterpaper]{article}
\usepackage[letterpaper,margin=1in,footskip=0.25in]{geometry}
\usepackage[utf8]{inputenc}
\usepackage{amsmath}
\usepackage{amsthm}
\usepackage{amssymb, pifont}
\usepackage{mathrsfs}
\usepackage{enumitem}
\usepackage{fancyhdr}
\usepackage{hyperref}

\pagestyle{fancy}
\fancyhf{}
\rhead{MAT 354}
\lhead{Assignment 2}
\rfoot{Page \thepage}

\setlength\parindent{24pt}
\renewcommand\qedsymbol{$\blacksquare$}

\DeclareMathOperator{\Qu}{\mathcal{Q}_8}
\DeclareMathOperator{\F}{\mathbb{F}}
\DeclareMathOperator{\T}{\mathcal{T}}
\DeclareMathOperator{\V}{\mathcal{V}}
\DeclareMathOperator{\U}{\mathcal{U}}
\DeclareMathOperator{\Prt}{\mathbb{P}}
\DeclareMathOperator{\R}{\mathbb{R}}
\DeclareMathOperator{\N}{\mathbb{N}}
\DeclareMathOperator{\Z}{\mathbb{Z}}
\DeclareMathOperator{\Q}{\mathbb{Q}}
\DeclareMathOperator{\C}{\mathbb{C}}
\DeclareMathOperator{\ep}{\varepsilon}
\DeclareMathOperator{\identity}{\mathbf{0}}
\DeclareMathOperator{\card}{card}
\newcommand{\suchthat}{;\ifnum\currentgrouptype=16 \middle\fi|;}

\newtheorem{lemma}{Lemma}

\newcommand{\tr}{\mathrm{tr}}
\newcommand{\ra}{\rightarrow}
\newcommand{\lan}{\langle}
\newcommand{\ran}{\rangle}
\newcommand{\norm}[1]{\left\lVert#1\right\rVert}
\newcommand{\inn}[1]{\lan#1\ran}
\newcommand{\ol}{\overline}
\newcommand{\ci}{i}
\begin{document}
\noindent
Q5: Using the binomial theorem, we expand: 
\begin{align*}
    (1+ \frac{z}{n})^n & = \sum_{k=0}^n {n \choose k} \cdot 1^{n-k} \frac{z^k}{n^k}
    \\ & = \sum_{k=0}^n \frac{n(n-1) \cdots (n-k+1)(n-k)!}{k! \cdot(n-k)!} \frac{z^k}{n^k}
    \\ & = \sum_{k=0}^n \frac{n(n-1)\cdots(n-k+1)}{n^k}\cdot \frac{z^k}{k!}
    \\ & = 1 + z + \sum_{k=2}^n \frac{n(n-1)\cdots(n-k+1)}{n^k}\cdot \frac{z^k}{k!}
    \\ & = 1+z+ \sum_{k=2}^n (1 - \frac{1}{n})\cdots ( 1 - \frac{k-1}{n}) \frac{z^k}{k!}
\end{align*}
As desired. Taking the limits, we get that $$\lim_{n \to \infty} (1+\frac{z}{n})^n = \lim_{n \to \infty} 1+z+ \sum_{k=2}^n (1 - \frac{1}{n})\cdots ( 1 - \frac{k-1}{n}) \frac{z^k}{k!} = \sum_{k=0}^n \frac{z^k}{k!}$$
Since as $n$ get arbitrarily large, the partial sums approach $\sum_{k=0}^n \frac{z^k}{k!}$. 
\end{document}