\documentclass[letterpaper]{article}
\usepackage[letterpaper,margin=1in,footskip=0.25in]{geometry}
\usepackage[utf8]{inputenc}
\usepackage{amsmath}
\usepackage{amsthm}
\usepackage{amssymb, pifont}
\usepackage{mathrsfs}
\usepackage{enumitem}
\usepackage{fancyhdr}
\usepackage{hyperref}

\pagestyle{fancy}
\fancyhf{}
\rhead{MAT 354}
\lhead{Assignment 2}
\rfoot{Page \thepage}

\setlength\parindent{24pt}
\renewcommand\qedsymbol{$\blacksquare$}

\DeclareMathOperator{\Qu}{\mathcal{Q}_8}
\DeclareMathOperator{\F}{\mathbb{F}}
\DeclareMathOperator{\T}{\mathcal{T}}
\DeclareMathOperator{\V}{\mathcal{V}}
\DeclareMathOperator{\U}{\mathcal{U}}
\DeclareMathOperator{\Prt}{\mathbb{P}}
\DeclareMathOperator{\R}{\mathbb{R}}
\DeclareMathOperator{\N}{\mathbb{N}}
\DeclareMathOperator{\Z}{\mathbb{Z}}
\DeclareMathOperator{\Q}{\mathbb{Q}}
\DeclareMathOperator{\C}{\mathbb{C}}
\DeclareMathOperator{\ep}{\varepsilon}
\DeclareMathOperator{\identity}{\mathbf{0}}
\DeclareMathOperator{\card}{card}
\newcommand{\suchthat}{;\ifnum\currentgrouptype=16 \middle\fi|;}

\newtheorem{lemma}{Lemma}

\newcommand{\tr}{\mathrm{tr}}
\newcommand{\ra}{\rightarrow}
\newcommand{\lan}{\langle}
\newcommand{\ran}{\rangle}
\newcommand{\norm}[1]{\left\lVert#1\right\rVert}
\newcommand{\inn}[1]{\lan#1\ran}
\newcommand{\ol}{\overline}
\newcommand{\ci}{i}
\begin{document}
\noindent
Q6: Let $\alpha \in \C$, $|z|<1$. Let $\sum_{k=0}^\infty a_n z^n = (1+z)^\alpha$. First, note that $1= (1+0)^\alpha = a_0$. We claim that each $a_n$ takes the form $$a_n = {\alpha \choose n }$$
We note that differentiating $n$ times, we get that $$\frac{\partial^n}{\partial z^n} (1+z)^\alpha = (\alpha)\cdot (\alpha-1) \cdots (\alpha-n+1)(1+z)^\alpha = \frac{\partial^n}{\partial z^n} \sum_{k=0}^\infty a_n z^n = \sum_{k=n}^\infty n! a_n z^{n-k}$$
At $z=0$ we have that $$(\alpha)(\alpha-1)\cdots(\alpha-n+1) = n! a_n$$
Since every term in the power series vanishes after $a_n$, and we conclude that $$a_n = {\alpha \choose n}$$
Therefore we have that $$(1+z)^\alpha = \sum_{k=0}^\infty {\alpha \choose n} z^n$$
\end{document}