\documentclass[12pt, a4paper]{article}
\usepackage[lmargin =0.5 in, 
rmargin=0.5in, 
tmargin=1in,
bmargin=0.5in]{geometry}
\geometry{letterpaper}
\usepackage{tikz-cd}
\usepackage{amsmath}
\usepackage{amssymb}
\usepackage{blindtext}
\usepackage{titlesec}
\usepackage{enumitem}
\usepackage{fancyhdr}
\usepackage{amsthm}
\usepackage{graphicx}
\usepackage{cool}
\usepackage{thmtools}
\usepackage{hyperref}
\graphicspath{ }					%path to an image

%-------- sexy font ------------%
%\usepackage{libertine}
%\usepackage{libertinust1math}

%\usepackage{mlmodern}				% very nice and classic
%\usepackage[utopia]{mathdesign}
%\usepackage[T1]{fontenc}


\usepackage{mlmodern}
\usepackage{eulervm}
%\usepackage{tgtermes} 				%times new roman
%-------- sexy font ------------%


% Problem Styles
%====================================================================%


\newtheorem{problem}{Problem}


\theoremstyle{definition}
\newtheorem{thm}{Theorem}
\newtheorem{lemma}{Lemma}
\newtheorem{prop}{Proposition}
\newtheorem{cor}{Corollary}
\newtheorem{fact}{Fact}
\newtheorem{defn}{Definition}
\newtheorem{example}{Example}
\newtheorem{question}{Question}

\newtheorem{manualprobleminner}{Problem}

\newenvironment{manualproblem}[1]{%
	\renewcommand\themanualprobleminner{#1}%
	\manualprobleminner
}{\endmanualprobleminner}

\newcommand{\penum}{ \begin{enumerate}[label=\bf(\alph*), leftmargin=0pt]}
	\newcommand{\epenum}{ \end{enumerate} }

% Math fonts shortcuts
%====================================================================%

\newcommand{\ring}{\mathcal{R}}
\newcommand{\N}{\mathbb{N}}                           % Natural numbers
\newcommand{\Z}{\mathbb{Z}}                           % Integers
\newcommand{\R}{\mathbb{R}}                           % Real numbers
\newcommand{\C}{\mathbb{C}}                           % Complex numbers
\newcommand{\F}{\mathbb{F}}                           % Arbitrary field
\newcommand{\Q}{\mathbb{Q}}                           % Arbitrary field
\newcommand{\PP}{\mathcal{P}}                         % Partition
\newcommand{\M}{\mathcal{M}}                         % Mathcal M
\newcommand{\eL}{\mathcal{L}}                         % Mathcal L
\newcommand{\T}{\mathbb{T}}                         % Mathcal T
\newcommand{\U}{\mathcal{U}}                         % Mathcal U\\
\newcommand{\V}{\mathcal{V}}                         % Mathcal V

% symbol shortcuts
%====================================================================%

\newcommand{\bd}{\partial}
\newcommand{\grad}{\nabla}
\newcommand{\lam}{\lambda}
\newcommand{\imp}{\implies}
\newcommand{\all}{\forall}
\newcommand{\exs}{\exists}
\newcommand{\delt}{\delta}
\newcommand{\ep}{\varepsilon}
\newcommand{\ra}{\rightarrow}
\newcommand{\vph}{\varphi}

\newcommand{\ol}{\overline}
\newcommand{\f}{\frac}
\newcommand{\lf}{\lfrac}
\newcommand{\df}{\dfrac}

% bracketting shortcuts
%====================================================================%
\newcommand{\abs}[1]{\left| #1 \right|}
\newcommand{\babs}[1]{\Big|#1\Big|}
\newcommand{\bound}{\Big|}
\newcommand{\BB}[1]{\left(#1\right)}
\newcommand{\dd}{\mathrm{d}}
\newcommand{\artanh}{\mathrm{artanh}}
\newcommand{\Med}{\mathrm{Med}}
\newcommand{\Cov}{\mathrm{Cov}}
\newcommand{\Corr}{\mathrm{Corr}}
\newcommand{\tr}{\mathrm{tr}}
\newcommand{\Range}[1]{\mathrm{range}(#1)}
\newcommand{\Null}[1]{\mathrm{null}(#1)}
\newcommand{\lan}{\langle}
\newcommand{\ran}{\rangle}
\newcommand{\norm}[1]{\left\lVert#1\right\rVert}
\newcommand{\inn}[1]{\lan#1\ran}
\newcommand{\op}[1]{\operatorname{#1}}
\newcommand{\bmat}[1]{\begin{bmatrix}#1\end{bmatrix}}
\newcommand{\pmat}[1]{\begin{pmatrix}#1\end{pmatrix}}
\newcommand{\vmat}[1]{\begin{vmatrix}#1\end{vmatrix}}

\newcommand{\amogus}{{\bigcap}\kern-0.8em\raisebox{0.3ex}{$\subset$}}
\newcommand{\Note}{\textbf{Note: }}
\newcommand{\Aside}{{\bf Aside: }}
%restriction
%\newcommand{\op}[1]{\operatorname{#1}}
%\newcommand{\done}{$$\mathcal{QED}$$}

%====================================================================%


\setlength{\parindent}{0pt}      	% No paragraph indentations
\pagestyle{fancy}
\fancyhf{}							% fancy header

\setcounter{secnumdepth}{0}			% sections are numbered but numbers do not appear
\setcounter{tocdepth}{2} 			% no subsubsections in toc

%template
%====================================================================%
%\begin{manualproblem}{1}
%Spivak.
%\end{manualproblem}

%\begin{proof}[Solution]
%\end{proof}

%----------- or -----------%

%\begin{problem} 		
%\end{problem}	

%\penum
%	\item
%\epenum
%====================================================================%


\newcommand{\Course}{MAT482}
\newcommand{\hwNumber}{3}

%preamble

\title{MAT482 HW3}
\author{Alexander Neagoe}
\date{\today}
\lhead{\Course A\hwNumber}
\rhead{\thepage}
%\cfoot{\thepage}


%====================================================================%
\begin{document}

\maketitle

\begin{problem}
\end{problem}
\penum
\item First we have that: 
\begin{align*}
	\frac{|f(x) g(x) - f(y)g(y)|}{|x-y|^\alpha}& = \frac{|f(x)g(x) + f(x)g(y)-f(x)g(y) - f(y)g(y)|}{|x-y|^\alpha}
	\\ & = \frac{|f(x) \left[  g(x) - g(y) \right]]  + g(y) \left[ f(x) - f(y)\right]|}{|x-y|^\alpha}
	\\ & \leq |f(x)| \frac{|g(x) - g(y)|}{|x-y|^\alpha} + |g(y)|\frac{|f(x) - f(y)|}{|x-y|^\alpha} \tag{By Triangle Inequality}
	\\ & \leq M_f \frac{|g(x) - g(y)|}{|x-y|^\alpha} + M_g \frac{|f(x)-f(y)|}{|x-y|^\alpha}\tag{By Continuity of $f,g$}
	\\ & 
\end{align*}
The above quantity is finite for all $x\neq y$ since $f,g\in C^\alpha$. We conclude that $fg\in C^\alpha$.
\item 
	Since $\{f_n\}$ is bounded in $C^\alpha$ it must be bounded in $C^0$ as well. Since $\norm{f_n}_{C^\alpha} \leq 1$ we have that for all $n$, $x\neq y\in \Omega$, 
	$$|f_n(x) - f_n(y)| \leq |x-y|^\alpha\implies |f_n(x) - f_n(y)| \leq M |x-y|,$$
Since H\"older Continuity implies  uniform continuity. Therefore $\{f_n\}$ is an equicontinuous family in $C^0$. By Arzela-Ascoli's Theorem there exists a subsequence $\{f_{n_k}\}$ so that $f_{n_k} \rightrightarrows f$ to some $f\in C^0$. 
We claim that $f\in C^\beta$. Since $C^\beta$ is a Banach Space, it is enough to show that $\{f_{n_k}\}$ is Cauchy. 
First relabel the sequence $\{f_{n_k}\}$ as $\{f_n\}$. By definition, we have:
$$\norm{f_n - f_m}_{C^\beta} = \sup_{\Omega} |f_m - f_n| + \sup_{x\neq y} \frac{|(f_n-f_m)(x) - (f_n-f_m)(y)|}{|x-y|^\beta}.$$
The first term can clearly be made less than $\ep$ just by uniform convergence. It remains to show the same is true for the second term. We compute:
\begin{align*}
	\sup_{x\neq y} \frac{|(f_n-f_m)(x) - (f_n-f_m)(y)|}{|x-y|^\beta} & = \left(\sup_{x\neq y} \frac{|(f_n-f_m)(x) - (f_n-f_m)(y)|}{|x-y|^\alpha} \right)^{\frac{\beta}{\alpha}} |(f_n-f_m)(x)-(f_n-f_m)(y)|^{1 - \frac{\beta}{\alpha}}
	\\ & \leq 2\left[f_n - f_m \right]^\frac{\beta}{\alpha}_{C^\alpha} \cdot \sup_{\Omega} |f_n-f_m|^{1 - \frac{\beta}{\alpha}}
	\\ & \leq 2^{1+ \frac{\beta}{\alpha}} \sup_\Omega |f_n - f_m|^{1 - \frac{\beta}{\alpha}} .\tag{By Triangle Inequality}
\end{align*}
We can also make the above quantity small than $\ep$ for sufficiently large $n,m$. The sequence is cauchy and thus converges in $C^\beta$. 
\epenum
\newpage
\begin{problem}
\end{problem}
\penum 
\item  
\begin{enumerate}[label = \roman*)]
	\item Since $\tilde{u}$ is a rescaled and translated $u$, we must have that $\tilde{u}$ is defined on $B_{1}(0)$ if and only if $u$ is defined on $B_{d_p}(p)$. Our selection of $d_p$ makes it so that $B_{d_p}(p) \subset \Omega$. So our function $\tilde{u}$ makes sense. 
	\item We compute a uniform bound on $\norm{\tilde{u}}_{C^2(B_{1/2}(0))}$. If $|x| < \frac{1}{2}$, we have that $d(p+d_p, \bd \Omega)>\frac{1}{2} d_p$. Thus we have
$$|D^2\tilde{u}| = M^{-1}d_p^2|D^2(p+d_p x)|\leq M^{-1} d_p^2 4 Md_p^{-2} = 4.$$
Where we use the fact that 
		$$|D^2u(p+d_p x)|\leq \frac{M}{d^2_{p+d_p x}}$$
In a similar fashion we compute :
		$$|D^2 \tilde{u}(x)| = |D^2 M^{-1} u(p+d_p x))| = M^{-1} d_p^2 |D^2u(p+d_p x)|.$$
At $x = 0$ we have that 
		$$|D^2\tilde{u}(0)| = M^{-1}d_p^2 |D^2u(p)| = 1.$$
	\item Using the chain rule we compute $a^{ij}\tilde{u}_{ij}$. 
		$$a^{ij}\tilde{u}_{ij} = M^{-1} a^{ij} (u(p+d_px))_{ij} = M^{-1}d_p^2 a^{ij}\tilde{u}_{ij} = M^{-1}d^2_p f(p + d_p x).$$
\item Since $|u|\leq 1$, 
	$$|\tilde{u}| = |M^{-1}u(p + dp_m x)|\leq M^{-1}. $$
\end{enumerate}
\item Suppose that lemma $0.2$ does not hold, that is we have for some function $u$ that for all $C$,
	$$\sup_{\Omega}d_x^2 |D^2u(x)| > C \left( \norm{f}_{C^\alpha}+ \norm{u}_{C^0}\right).$$
We can find a sequence $\{u_k\}$ so that if $C=m$, $a^{ij}(u_m)_{ij} = f_m$, 
$$\sup_{\Omega} d_x^2 |D^2u_m(x)| > k \left(\norm{f_m}_{C^\alpha} + \norm{u}_{C^0} \right).$$
Let $p_m$, $M_m$ be such that
$$\sup_{\Omega} d_x^2 |D^2u_m| = d_{p_m}^2 |D^2u_m(p_m)| = M_m.$$
By hypothesis, we must have that $M_m \to \infty$ as $m \to \infty$. Define $\tilde{u}_m = M_m^{-1}u_m(p_m + xdp_m)$. All of the results from part $a)$ hold, in particular $\norm{u_m}_{C^2(B_{1/2}(0)}$ is uniformly bounded, and $|u_m| \leq 1$ on $B_1(0)$. We have that $a^{ij}(\tilde{u})_{ij} = f_m(p_m + dp_m x)$. So by Theorem 0.1, we have:
$$(\min\{d_x, d_y\} )^\alpha \frac{\left|D^2 \tilde{u}_m(x) - D^2\tilde{u}_mu(y) \right|}{|x-y|^\alpha}\leq C\left(\norm{f_m}_{C^\alpha(\Omega^\prime)} + \norm{\tilde{u}_m}_{C^2(\Omega^\prime)} \right).$$
By taking the $\sup$ over $x,y\in B_{1/2}(0)$, we get that 
$$\sup_{x\neq y}\frac{\left|D^2\tilde{u}_m(x) - D^2 \tilde{u}_m(y) \right|}{|x-y|^\alpha}\leq C_1.$$
Since the $\tilde{u}_m$ are uniformly bounded in $C^2$, and have holder constant $C_1$ they must be in $C^{2,\alpha}$. Therefore $\{\tilde{u}_m\}$ is bounded. By Arzela-Ascoli, we can find a convergent subsequence, $\{\tilde{u}_{m_k}\}$ with limit $\tilde{u}_\infty$. We have that 
$$\norm{\tilde{u}_\infty}_{C^0} = \lim_{m_k \to \infty}\norm{\tilde{u}_{m_k}}_{C^0} \leq \lim_{m_k \to \infty} M_{m_k}^{-1} = 0.$$
However,
$$|D^2\tilde{u}_\infty(0)| = \lim_{m_k \to \infty} |D^2\tilde{u}_{m_k}(0)| = 1.$$
This is a contradiction. 
\epenum
\newpage
\begin{problem}
\end{problem}
Since $\ol{u}$ agrees with a harmonic function on the upper and lower half planes, it is enough to show that it is harmonic along $x_n= 0$. Since $\ol{u}$ is continuous, we check that it has mean value property for $x_n = 0$. Take a point $x = (x_1, \dots , x_{n-1} , 0)$. We compute: 
\begin{align*}
	\frac{1}{\omega_n r^n} \int_{B_r(x)} \ol{u}(y) dy & = \frac{1}{\omega_n r^n} \left[\int_{B_r(x)\cap \{x_n >0\}} \ol{u}(y) dy + \int_{B_r\cap\{ x_n <0\}} \ol{u}(y) dy \right]
	\\ & = \frac{1}{\omega_n r^n} \left[ \int_{B_r\cap \{x>0\}} u(y)dy + \int_{B_r(x) \cap \{x_n<0\}} -u(y_1, \dots , -y_n)dy \right]
	\\ & = \frac{1}{\omega_n r^n} \left[ \int_{B_r\cap \{x>0\}} u(y)dy + \int_{B_r(x) \cap \{x_n >0\}} -u(y) dy  \right] \tag{Change of Variables}
	\\ & = 0 
	\\ & = u(x)
\end{align*}
So $u$ is continuous, has mean value property, and agrees everywhere with a harmonic function. We conclude $u$ is harmonic. 
\newpage
\begin{problem}
\end{problem}
\penum
\item Since $\norm{f}_{C^\alpha} + \norm{u}_{C^2} + \norm{\phi}_{C^\alpha,2}$ we must have that $\norm{f}_{C^\alpha} + \norm{u}_{C^2} \leq 1$. By theorem 0.1 we have that 
	$$\left( \min \{d_{p_m} ,d_{q_m} \}\right)^\alpha \frac{|D^2u(p_m) - D^2u(q_m)| }{|p_m-q_m|^\alpha} \leq C \implies d_{p_m}^\alpha M \leq C \implies d_{p_m}^\alpha \leq CM^{-1}.$$
Since $\norm{u}_{C^2} \leq 1$, we must have that by triangle inequality:
$$|D^2u(p_m) - D^2u(q_m)|\leq 2.$$
Multiplying both sides by $\frac{r_m^\alpha}{r_m^\alpha}$, we get that:
$$r^\alpha_m \frac{|D^2u(p_m) - D^2u(q_m)|}{r_m^\alpha}\leq 2 \implies r_m^\alpha M \leq 2 \implies r_m^\alpha \leq 2M^{-1}.$$
Since $M \geq m$, as $m \to \infty$ we have that $d_{p_m}^\alpha, r_m^\alpha \to 0$. 
\item 
\begin{enumerate}[label = \roman*) ]
	\item Note that $\tilde{v}_m$ is a sum of $\tilde{u}_m$ and a polynomial in $x$ along with some constant terms. Therefore it will be defined exactly where $\tilde{u}_m$ is defined. Since $u_m$ is defined on $B_1(e_n)$, we must have that $\tilde{v}_m$ is defined on the ball of radius $1/r_m$ centered about $e_n$. Thus we wish to show that if $x\in \Gamma_m$, then $(r_mx_n - 1)^2 + \sum_{i}^{n-1}(r_mx_i)^2 \leq 1$. 
We have that 
		$$-1 + \sum_{i}^{n-1} (r_mx_i)^2 \leq r_mx_n - 1 \leq 0.$$
Squaring and flipping the directions of the inequalities, we have that 
$$ \left(-1 + \sum_{i}^{n-1} (r_mx_i)^2  \right)^2 \geq (r_m x_n- 1)^2 \geq 0. $$
Adding $\sum_{i}^{n-1} (r_m x_i)^2$ to both sides we get that:
		$$1 - \sum_{i}^{n-1} (r_mx_i)^2  + \left(\sum_{i}^{n-1} (r_mx_i)^2 \right)^2 \geq (r_mx_n-1)^2 + \sum_{i}^{n-1}(r_mx_i)^2.$$
Since $\sum_{i}^{n-1} (r_mx_i)^2 \leq 1/2$, the lefthand side is less than 1. 
\item We have $v_m(x) =  \tilde{u}_m(x) - \tilde{u}_m(0) + - \sum_i x_i \frac{\tilde{u}_m(0)}{\partial x_i}  - \frac{1}{2} \sum_{i,j} \frac{\partial^2\tilde{u}_m}{\partial x_i \partial x_j}(0) x_ix_j.$
It is easy to see that 
$$v_m(0) = \tilde{u}_m(0) - \tilde{u}_m(0) = 0.$$
As well as
$$Dv_m(0) = D\tilde{u}_m(0) - D\tilde{u}_m(0) =0 ,$$
since the degree 2 polynomial just evaluates to $0$, and the linear term has a gradient of $D\tilde{u}_m(0)$.  
Finally we have that 
$$D^2 v_m(0) = D^2\tilde{u}_m(0) - D^2 \tilde{u}_m(0). $$
This is since the constant and linear terms vanish and the hessian of the quadratic term is exactly $D^2\tilde{u}_m(0)$. Furthermore for $x,y\in \Gamma_m$, we have:
\begin{align*}
 |D^2 v_m(x) - D^2v_m(y)| & = |D^2\tilde{u}_m(x) - D^2\tilde{u}_m(y)|
 \\ & = |D^2(M^{-1}r_m^{-2-\alpha}u(r_m x)) - D^2(M^{-1}r_m^{-2-\alpha}u(r_m y))|
 \\ & = M^{-1}r_m^{-\alpha}|D^2u_m(r_mx) - D^2u_m(r_my)|
 \\ & \leq |x-y|^\alpha \tag{by assumption at points $r_mx,r_my$}
\end{align*}
\item We first claim that $\frac{p_m}{r_m},\frac{q_m}{r_m}\in B_{\frac{dp_m}{r_m}+1}(0)$.
	Since we have rotated the sphere so that $p_m = (0, \dots , 0, dp_m)$, so $\frac{p_m}{r_m}$ belongs to the ball. Furthermore since $|p_m - q_m| = r_m$ we have that $\left|\frac{p_m}{r_m} - \frac{p_m}{r_m} \right| = 1,$ so by triangle inequality $\frac{q_m}{r_m}$ belongs to the ball as well.
We see that 
		$$\left|D^2v_m(x_m) - D^2 v_m(y_m) \right| = M^{-1}r_m^{-\alpha}\left|D^2u_m(p_m) - D^2u_m(q_m) \right| = 1.$$
	\item For $x,y\in\bd \Omega_m$  compute that: 
\begin{align*}
	\frac{\left|D_{T_i}D_{T_j}v_m(x) - D_{T_i} D_{T_j}v_m(y) \right|}{|x-y|^\alpha}  & = M^{-1}\frac{|D_{T_i} D_{T_j}u_m(x) - D_{T_i} D_{T_j} u(y)  |}{|x-y|^\alpha} \tag{By definition of $v_m$}
	\\ & = M^{-1} \frac{|D_{T_i}D_{T_j} \phi_m(x) - D_{T_i} D_{T_j} \phi_m(y) |}{|x-y|^\alpha} \tag{since $x,y\in \bd \Omega$}
	\\ & \leq M^{-1} \tag{By assumption}
\end{align*}
\item We first determine second order derivatives of $v_m$. 
$${v_m(x)}_{ij} =M^{-1}r_m^{-\alpha} \left(u_{ij}(r_mx) - u_m(0) \right). $$
It follows that $$a^{ij} \partial_i \partial_j v_m(x) = M^{-1}r_m^{-\alpha} \left(f_m(r_mx) - a^{ij}_m ({u_m})_{ij}(0) \right).$$
On the boundary, we have that
		$$v_m |_{\bd \Omega}(x) = M^{-1} r_m^{-2-\alpha} \left( \phi_m(r_m x) - \phi_m(0)\right)  -M^{-1}r_m^{-1-\alpha} \sum_{i}^{n} x_i (u_m )_i(0) -\frac{M^{-1} r_m^{-\alpha}}{2} \sum_{i,j} (u_m)_{ij}(0) x_i x_j$$
\end{enumerate}
\item By $1b)$ we have a uniform $C^{2,\alpha}$ bound on the sequence $\{v_m\}$. We can therefore pass to a uniformly convergent subsequence, and relabel it as $\{v_m\}$. Since $M^{-1} \to 0$, by $ii)$ we have that $a^{ij}(v_m(x))_{ij} \to 0$. Therefore the limit function $v_\infty$ is harmonic up to a change of variables.
Furthermore as $M^{-1} \to 0$ we have that $v_\infty(x) = 0$  when $x_n =0$ since $v_m$ is uniformly bounded on the boundary. Finally note that the this locally looks like the half plane, since we can zoom in sufficiently close on the boundary of the ball. Therefore we can apply the Schwartz reflection principle and get a harmonic function which is $0$ on $x_n =0$. But by part $iii)$ we have that 
$$|D^2 v_\infty(x) - D^2v_\infty(y)| = 1$$
at some $x,y$ which lie in the ball. This is a contradiction. 
\epenum
\newpage
\begin{problem}
\end{problem}
\penum
\item First note that for $L_t$ will have coefficients of $(1-t)\delta_{ij} + ta^{ij}$ which are uniformly bounded in $C^{\alpha}$ by a constant depending on $n,\lambda, \norm{a^{ij}}_{C^\alpha}$.
Therefore $\norm{L_tu}_{C^\alpha} \leq C_1 \norm{u}_{C^\alpha}$. 
Next note that by theorem 0.4, we have a constant $C_{L_t}$  depending on $\lambda, n,\Omega$ and $\norm{a^{ij}}_{C^\alpha(\ol{B})}$ for each $L_t$. The ellipticity constants for each $L_t$ will be bounded below by $\min\{1,\lambda\}$ and bounded above by $\max\{1,\Lambda\}$. Thus $C_t$ will be bounded above by some $C_2$ depending on $\lambda,\Lambda, n, B$. We proceed by induction. For $k=0$, since $f\in C^\alpha(\ol{B})$, we have that $u\in C^{2, \alpha}(\ol{B})$. We have that
	$$\norm{u_0}_{C^{2, \alpha}} \leq C_2 \left( \norm{f}_{C^{\alpha}(\ol{B})} + \norm{u_0}_{C^0 (\ol{B}} \right) \leq C_2(1+C_1)\left( \norm{f}_{C^{\alpha}(\ol{B})} + \norm{u_0}_{C^0 (\ol{B}} \right). $$
 We have proven in class that the following bound holds: 
$$\norm{u_0}_{C^0(B)} \leq \norm{u|_{\bd B}}_{\bd B} + C_t \norm{f}_{C^0(B)}.$$
Since $u_0$ vanishes along the boundary, we have that 
$$\norm{u_0}_{C^0(\ol{B})}\leq C_t\norm{f}_{C^0(B)} \leq C_t\norm{f}_{C^\alpha(\ol{B})}.$$ 
For some constant $C_t$ depending on $n , \lambda , \norm{(1-t)\delta_{ij} - t a^{ij}}_{C^\alpha}, B$. A similar argument as above shows that we can take a $C_3$ uniformly bounding $C_t$. Therefore we must have that 
$$\norm{u_0}_{C^{2,\alpha} (\ol{B})} \leq C_2(1+C_1)(1+C_3)\norm{f}_{C^\alpha(\ol{B})} = C\norm{f}_{C^\alpha}$$ 
Now suppose that the result holds for $0, \dots , k$. Then we must have that $f - \sum_{i=0}^k Lu_i \in C^\alpha(\ol{B}))$ and $\Delta u_{k+1} = (\Delta - L)u_k = f - \sum_{i=0}^k Lu_i$. Therefore $u_{k+1} \in C^{2,\alpha}(\ol{B})$. By base case we have that 
$$\norm{u_{k+1}}_{C^{2,\alpha}(\ol{B})}\leq C\norm{u_k}_{C^{2,\alpha}(\ol{B})}\leq C^{k+1}\norm{f}_{C^{\alpha}(B)}.$$
\item We can write: 
\begin{align*}L_t v_k &= (1-t)\Delta v_k + t Lv_k 
	\\ & = \sum_{j=0}^k t^j ((1-t)\Delta + t L)u_j
	\\ & = \sum_{j=0}^k t^j \Delta u_j - t^{j+1} (\Delta - L) u_j
	\\ & = \sum_{j=0}^k t^j \Delta u_j - t^{j+1} \Delta u_{j+1} \tag{By definition}
	\\ & = \Delta u_0 - t^{k+1}\Delta u_{k+1} \tag{Telescoping the sum}
	\\ & = f - t^{k+1}(\Delta - L)u_k
\end{align*}
\item For $n>m$, by $a)$ we have 
$$\norm{v_n(t) - v_m(t)}_{C^2,\alpha} \leq \sum_{j = m+1} t^j \norm{u_j}_{C^{2, \alpha}}\leq \norm{f}_{C^\alpha} \sum_{m+1}^k (tC)^j = \norm{f}_{C^\alpha} \frac{tC\left(t^kC^k - t^mC^m\right)}{tC- 1}.$$
Taking $t_0 = \frac{1}{2C}$ for $ t \leq t_0$ the above becomes arbitrarily small as $m,n \to \infty$. Therefore the sequence $\{v_n(t)\}$ is Cauchy and converges in $C^{2,\alpha}$ when $t \leq t_0$. Now let $v_{\infty,t}$ be the limit of the sequence at $t$.
It remains to show that $v_\infty(t)$ solves
$$\begin{cases}
L_t v_{\infty, t} &= f \text{ in $B$}
\\ v_{\infty,t}|_{\bd B} &= 0.
\end{cases}$$ 
Since each $v_n(t)$ is $0$ on $\bd B$ we have that $v_{\infty, t}$ is 0 on the boundary of $B$ as well. By $b)$, we have
$$\norm{L_t v_{\infty, t} - f}_{C^\alpha} \leq \norm{L_t v_{\infty , t} - L_t v_n}_{C^\alpha} + \norm{L_t v_n - f}_{C^\alpha} = \norm{L_t v_{\infty , t} - L_t v_n}_{C^\alpha}  + t^{k+1} \norm{(L-\Delta) u_n}_{C^\alpha}.$$
The $a^{ij}$ belong to $C^\alpha$ so we can find constants $C_1,C_2$ so that 
$$C_1\norm{L_t v_{\infty , t} - L_t v_n}_{C^\alpha}  +C_2 t^{k+1} \norm{(L-\Delta) u_n}_{C^\alpha}\leq C_1 \norm{v_{\infty, t} - v_n(t)}_{C^{2,\alpha}} + (tC)^{k+1}C_2 \norm{f}_{C^\alpha}.$$
This quantity will go to $0$ as $n\to \infty$ so we have that $L_t v_{\infty,t} = f$. 
\item By part $c)$, the equation 
$$\begin{cases}
	L_{t_0} u &= f \text{ in $B$}
	\\ u|_{\bd B} &= 0.
\end{cases}$$ has a solution in $C^{2,\alpha}$ for any $f\in C^\alpha$. We can inductively define:
$$\begin{cases}
	L_{t_0} u_k&= (\Delta - L)u_{k-1} \text{ in $B$}
	\\ u_k|_{\bd B} &= 0.
\end{cases}$$ 
so that we can get the same result as in  $a)$ with the same $C$. Therefore we can repeat the arguments of $b),c)$ and get that $v_k$ converges to a solution of 
$$\begin{cases}
	L_t v_{\infty, t} &= f \text{ in $B$}
	\\ v_{\infty,t}|_{\bd B} &= 0.
\end{cases}$$ 
as long as $t-t_0 \leq t_0$. Thus we can solve when $t\leq 2t_0$, and iterating finitely many times will solve $(*)$. 
\epenum
\end{document}
